refacotored

Primitive_Matchers/No_Spoof.thy
@@ -1,6 +1,7 @@
 theory No_Spoof
 imports Common_Primitive_Matcher
   "../Common/Negation_Type_DNF"
+        Primitive_Normalization
 begin
 
 section{*No Spoofing*}
@@ -28,9 +29,15 @@ section{*No Spoofing*}
   interface and is allowed by the firewall must be in the IP range of that interface.
   *}
   definition no_spoofing :: "ipassignment \<Rightarrow> common_primitive rule list \<Rightarrow> bool" where
-    "no_spoofing ipass rs \<equiv> \<forall> iface \<in> dom ipass.  \<forall>p.
+    "no_spoofing ipassmt rs \<equiv> \<forall> iface \<in> dom ipassmt. \<forall>p.
         ((common_matcher, in_doubt_allow),p\<lparr>p_iiface:=iface_sel iface\<rparr>\<turnstile> \<langle>rs, Undecided\<rangle> \<Rightarrow>\<^sub>\<alpha> Decision FinalAllow) \<longrightarrow>
-            p_src p \<in> (\<Union>(base, len) \<in> the (ipass iface). ipv4range_set_from_bitmask base len)"
+            p_src p \<in> (ipv4cidr_union_set (the (ipassmt iface)))"
+
+  (*should be sound:
+      if no_spoofing certifies your ruleset, then your ruleset prohibits spoofing
+    may not be complete:
+      no_spoofing may return False even though your ruleset prevents spoofing
+      (should only occur if some strange and unknown primitives occur)*)
 
 (*
 and now code to check this ....
@@ -39,11 +46,67 @@ and now code to check this ....
   collect all src_ips allowed for a specific iiface?
   check collected src_ips subseteq ipassignment(iface)
 *)
+(*
+  definition get_matching_src_ips :: "common_primitive match_expr \<Rightarrow> ipv4addr set" where
+    "get_matching_src_ips m \<equiv> \<Union> ips \<in> set (fst (primitive_extractor (is_Src, src_sel) m)).  
+                                  (case ips of Pos ip \<Rightarrow> ipv4s_to_set ip | Neg ip \<Rightarrow> - ipv4s_to_set ip)"
+                (*todo: primitive extractor and 32wordinterval?*)
 
-  fun no_spoofing_algorithm :: "iface \<Rightarrow> ipassignment \<Rightarrow> common_primitive rule list \<Rightarrow> (ipv4addr \<times> nat) set \<Rightarrow> bool" where
-    "no_spoofing_algorithm iface ipassmt [] allowed = (ipv4cidr_union_set allowed \<subseteq> ipv4cidr_union_set (the (ipassmt iface)))" |
-    "no_spoofing_algorithm iface ipassmt ((Rule m a)#rs) allowed = True(*(if iface_matches iface m then
-        no_spoofing_algorithm iface ipassmt rs (allowed \<union> *)" (*probably have allowed and denied set? Start with UNIV or {}?*)
+                (* only makes sense if there is a packet which can match*)
+
+  (*TODO: action!*)
+  lemma "normalized_nnf_match m \<Longrightarrow> get_matching_src_ips m = {ip. \<exists>p. matches (common_matcher, in_doubt_allow) m a (p\<lparr>p_src:= ip\<rparr>)}"
+    unfolding get_matching_src_ips_def
+    apply(rule Set.equalityI)
+     apply(safe)
+     apply(cases "primitive_extractor (is_Src, src_sel) m")
+     apply(frule_tac p="p\<lparr>p_src:= x\<rparr>" in primitive_extractor_correct(1)[OF _ wf_disc_sel_common_primitive(3), where \<gamma>="(common_matcher, in_doubt_allow)" and a=a])
+      apply(simp)
+     apply(simp)
+     apply(simp split: negation_type.split_asm)
+    oops
+
+  definition in_iface_matches :: "iface \<Rightarrow> common_primitive match_expr \<Rightarrow> bool" where
+    "in_iface_matches iiface m = True" (*todo: primitive extractor and (match_iface i (p_iiface p)) for any packet?*)
+      (*ANY packet? well any with iiface, this should be straight forward*)
+
+  (*TODO: verify this algorithm first*)
+  fun no_spoofing_algorithm :: "iface \<Rightarrow> ipassignment \<Rightarrow> common_primitive rule list \<Rightarrow> ipv4addr set \<Rightarrow> ipv4addr set \<Rightarrow> bool" where
+    "no_spoofing_algorithm iface ipassmt [] allowed denied \<longleftrightarrow> 
+      (allowed - denied) \<subseteq> ipv4cidr_union_set (the (ipassmt iface))" |
+    "no_spoofing_algorithm iface ipassmt ((Rule m Accept)#rs) allowed denied = (if in_iface_matches iface m
+        then
+          no_spoofing_algorithm iface ipassmt rs (allowed \<union> {ip. \<exists>p. matches (common_matcher, in_doubt_allow) m Accept (p\<lparr>p_src:= ip\<rparr>)}) denied
+        else
+          no_spoofing_algorithm iface ipassmt rs allowed denied)" |
+    "no_spoofing_algorithm iface ipassmt ((Rule m Drop)#rs) allowed denied = (if in_iface_matches iface m
+        then
+          no_spoofing_algorithm iface ipassmt rs allowed (denied \<union> {ip. \<exists>p. matches (common_matcher, in_doubt_allow) m Drop (p\<lparr>p_src:= ip\<rparr>)})
+        else
+          no_spoofing_algorithm iface ipassmt rs allowed denied)"  |
+    "no_spoofing_algorithm _ _ _ _ _ = undefined"
+
+  (*implementation could store ipv4addr set as 32 wordinterval*)
 
 
+  definition "nospoof iface ipassmt rs = (\<forall>p.
+          (approximating_bigstep_fun (common_matcher, in_doubt_allow) (p\<lparr>p_iiface:=iface_sel iface\<rparr>) rs Undecided = Decision FinalAllow) \<longrightarrow>
+              p_src p \<in> (ipv4cidr_union_set (the (ipassmt iface))))"
+  definition "setbydecition iface rs dec = {ip. \<exists>p. approximating_bigstep_fun (common_matcher, in_doubt_allow) 
+                           (p\<lparr>p_iiface:=iface_sel iface, p_src := ip\<rparr>) rs Undecided = Decision dec}"
+  lemma "simple_ruleset rs2 \<Longrightarrow>
+        iface \<in> dom ipassmt \<Longrightarrow>
+        allowed = setbydecition iface rs1 FinalAllow \<Longrightarrow>
+        denied = setbydecition iface rs1 FinalDeny \<Longrightarrow>
+        no_spoofing_algorithm iface ipassmt rs2 allowed denied \<longleftrightarrow> 
+        nospoof iface ipassmt (rs1@rs2)"
+  apply(induction iface ipassmt rs2 allowed denied arbitrary: rs1 allowed denied rule: no_spoofing_algorithm.induct)
+          apply(simp_all add: simple_ruleset_def)
+    apply(simp add: setbydecition_def nospoof_def)
+    defer
+    apply safe
+    apply(simp_all)
+    
+  oops
+*)
 end
