Semantics_Ternary/Matching_Ternary.thy
@@ -88,9 +88,8 @@ lemma matches_casesE:
     (ternary_ternary_eval (map_match_tac \<beta> p m) = TernaryUnknown \<Longrightarrow> \<alpha> a p \<Longrightarrow> P) \<Longrightarrow> 
     (ternary_ternary_eval (map_match_tac \<beta> p m) = TernaryTrue \<Longrightarrow> P)
   \<Longrightarrow> P"
-apply(induction m)
-apply(auto split: option.split_asm simp: matches_case_tuple ternary_eval_def ternary_to_bool_bool_to_ternary elim: ternary_to_bool.elims)
-done
+proof(induction m)
+qed(auto split: option.split_asm simp: matches_case_tuple ternary_eval_def ternary_to_bool_bool_to_ternary elim: ternary_to_bool.elims)
 
 
 text{*
@@ -107,8 +106,8 @@ lemma bunch_of_lemmata_about_matches:
   "matches (\<beta>, \<alpha>) (Match expr) a p = (case ternary_to_bool (\<beta> expr p) of Some r \<Rightarrow> r | None \<Rightarrow> (\<alpha> a p))" (*Match raw*)
   "matches (\<beta>, \<alpha>) (Match expr) a p = (case (\<beta> expr p) of TernaryTrue \<Rightarrow> True | TernaryFalse \<Rightarrow> False | TernaryUnknown \<Rightarrow> (\<alpha> a p))" (*Match raw explicit*)
   "matches \<gamma> (MatchNot (MatchNot m)) a p \<longleftrightarrow> matches \<gamma> m a p" (*idempotence*)
-apply(case_tac [!] \<gamma>)
-by (simp_all split: ternaryvalue.split add: matches_case_ternaryvalue_tuple)
+proof(case_tac [!] \<gamma>)
+qed (simp_all split: ternaryvalue.split add: matches_case_ternaryvalue_tuple)
 
 
 (*kind of the DeMorgan Rule for matches*)
@@ -162,12 +161,10 @@ lemmas matches_dest = matches_simp2 matches_simp22
 
 
 lemma matches_iff_apply_f_generic: "ternary_ternary_eval (map_match_tac \<beta> p (f (\<beta>,\<alpha>) a m)) = ternary_ternary_eval (map_match_tac \<beta> p m) \<Longrightarrow> matches (\<beta>,\<alpha>) (f (\<beta>,\<alpha>) a m) a p \<longleftrightarrow> matches (\<beta>,\<alpha>) m a p"
-  apply(simp split: ternaryvalue.split_asm ternaryvalue.split add: matches_case_ternaryvalue_tuple)
-  done
+  by(simp split: ternaryvalue.split_asm ternaryvalue.split add: matches_case_ternaryvalue_tuple)
 
 lemma matches_iff_apply_f: "ternary_ternary_eval (map_match_tac \<beta> p (f m)) = ternary_ternary_eval (map_match_tac \<beta> p m) \<Longrightarrow> matches (\<beta>,\<alpha>) (f m) a p \<longleftrightarrow> matches (\<beta>,\<alpha>) m a p"
-  apply(simp split: ternaryvalue.split_asm ternaryvalue.split add: matches_case_ternaryvalue_tuple)
-  done
+  by(simp split: ternaryvalue.split_asm ternaryvalue.split add: matches_case_ternaryvalue_tuple)
 
 
 
@@ -287,9 +284,7 @@ lemma[code_unfold]: "remove_unknowns_generic \<gamma> a (MatchNot (MatchAnd m1 m
      else
         MatchNot (MatchAnd (MatchNot m1') (MatchNot m2')))
        )"
-apply(cases \<gamma>)
-apply(simp)
-done
+by(cases \<gamma>)(simp)
 
 
 lemma remove_unknowns_generic_simp_3_4_unfolded: "remove_unknowns_generic (\<beta>, \<alpha>) a (Match A) = (if
@@ -354,9 +349,10 @@ definition packet_independent_\<beta>_unknown :: "('a, 'packet) exact_match_tac 
 
 lemma remove_unknowns_generic_specification: "a = Accept \<or> a = Drop \<Longrightarrow> packet_independent_\<alpha> \<alpha> \<Longrightarrow> packet_independent_\<beta>_unknown \<beta> \<Longrightarrow>
    \<not> has_unknowns \<beta> (remove_unknowns_generic (\<beta>, \<alpha>) a m)"
-  apply(induction "(\<beta>, \<alpha>)" a m rule: remove_unknowns_generic.induct)
-        apply(simp_all)
-   apply(simp_all add: packet_independent_unknown_match packet_independent_\<beta>_unknown_def)
-   done
+  proof(induction "(\<beta>, \<alpha>)" a m rule: remove_unknowns_generic.induct)
+  case 3 thus ?case by(simp add: packet_independent_unknown_match packet_independent_\<beta>_unknown_def)
+  next
+  case 4 thus ?case by(simp add: packet_independent_unknown_match packet_independent_\<beta>_unknown_def)
+  qed(simp_all)
 
 end
